implement most of slabs deallocation,
some remaining admits
size class deallocation remaining too

src/Slabs2.fst
@@ -25,66 +25,190 @@ open Slots
 open Slots2
 open Slabs
 
-//TODO: remove, now likely useless
-//let deallocate_slab_aux
-//  (size_class: sc)
-//  (partial_slabs_ptr empty_slabs_ptr full_slabs_ptr: ref SL.t)
-//  (partial_slabs empty_slabs full_slabs: SL.t)
-//  (slab: array U8.t{A.length slab = U32.v page_size})
-//  (md: slab_metadata)
-//  (ptr: array U8.t)
-//  : Steel bool
-//  (
-//    A.varray ptr `star`
-//    slab_vprop size_class slab md `star`
-//    vptr empty_slabs_ptr `star`
-//    SL.llist (p_empty size_class) empty_slabs `star`
-//    vptr partial_slabs_ptr `star`
-//    SL.llist (p_partial size_class) partial_slabs `star`
-//    vptr full_slabs_ptr `star`
-//    SL.llist (p_full size_class) full_slabs
-//  )
-//  (fun b ->
-//    (if b then emp else A.varray ptr) `star`
-//    SL.ind_llist (p_empty size_class) empty_slabs_ptr `star`
-//    SL.ind_llist (p_partial size_class) partial_slabs_ptr `star`
-//    SL.ind_llist (p_full size_class) full_slabs_ptr
-//  )
-//  (requires fun h0 ->
-//    let diff = A.offset (A.ptr_of ptr) - A.offset (A.ptr_of slab) in
-//    same_base_array slab ptr /\
-//    0 <= diff /\
-//    diff <= U32.v page_size - U32.v size_class /\
-//    (U32.v page_size) % (U32.v size_class) = 0 /\
-//    sel partial_slabs_ptr h0 == partial_slabs /\
-//    sel empty_slabs_ptr h0 == empty_slabs /\
-//    not (SL.is_null_t partial_slabs))
-//  (ensures fun _ _ _ -> True)
-//  =
-//  let r = deallocate_slot size_class md slab ptr in
-//  if r
-//  then (
-//    // cf Slack discussion: flattening bijectively the lists is required
-//    sladmit ();
-//    SL.pack_ind (p_partial size_class) partial_slabs_ptr partial_slabs;
-//    SL.pack_ind (p_empty size_class) empty_slabs_ptr empty_slabs;
-//    return r
-//  ) else (
-//    sladmit ();
-//    SL.pack_ind (p_partial size_class) partial_slabs_ptr partial_slabs;
-//    SL.pack_ind (p_empty size_class) empty_slabs_ptr empty_slabs;
-//    return r
-//  )
-
 open FStar.Mul
 open SteelStarSeqUtils
 open SteelVRefineDep
 module AL = ArrayList
+module ALG = ArrayListGen
 
 unfold
 let blob = Slabs.blob
 
-assume val deallocate_slab_aux_empty
+#push-options "--z3rlimit 75 --compat_pre_typed_indexed_effects"
+let deallocate_slab_aux_cond
+  (size_class: sc)
+  (md: slab_metadata)
+  (arr: array U8.t{A.length arr = U32.v page_size})
+  : Steel bool
+  (slab_vprop size_class arr md)
+  (fun _ -> slab_vprop size_class arr md)
+  (requires fun _ -> True)
+  (ensures fun h0 r h1 ->
+    let blob0
+      : t_of (slab_vprop size_class arr md)
+      = h0 (slab_vprop size_class arr md) in
+    let blob1
+      : t_of (slab_vprop size_class arr md)
+      = h1 (slab_vprop size_class arr md) in
+    let v0 : Seq.lseq U64.t 4 = dfst (fst blob0) in
+    dfst (fst blob0) == dfst (fst blob1) /\
+    dsnd (fst blob0) == dsnd (fst blob1) /\
+    blob0 == blob1 /\
+    r == is_empty size_class v0
+  )
+  =
+  assert (t_of (A.varray md) == Seq.lseq U64.t 4);
+  let md_as_seq : G.erased (Seq.lseq U64.t 4)
+    = elim_slab_vprop size_class md arr in
+  let r = is_empty_s size_class md in
+  intro_slab_vprop size_class md md_as_seq arr;
+  return r
+
+inline_for_extraction noextract
+let deallocate_slab_aux_1_partial
+  (size_class: sc)
+  (slab_region: array U8.t{A.length slab_region = U32.v metadata_max * U32.v page_size})
+  (md_bm_region: array U64.t{A.length md_bm_region = U32.v metadata_max * 4})
+  (md_region: array AL.cell{A.length md_region = U32.v metadata_max})
+  (md_count: ref U32.t)
+  (r1 r2 r3: ref US.t)
+  (md_count_v: U32.t{U32.v md_count_v <= U32.v metadata_max})
+  (md_region_lv: G.erased (Seq.lseq AL.status (U32.v md_count_v)))
+  (idx1: US.t)
+  (idx2: US.t)
+  (idx3: US.t)
+  (pos: US.t{US.v pos < U32.v md_count_v})
+  : Steel unit
+  (
+    vptr md_count `star`
+    vptr r1 `star`
+    vptr r2 `star`
+    vptr r3 `star`
+    (AL.varraylist pred1 pred2 pred3
+      (A.split_l md_region (u32_to_sz md_count_v))
+      (US.v idx1) (US.v idx2) (US.v idx3)) `star`
+    starseq
+      #(pos:U32.t{U32.v pos < U32.v md_count_v})
+      #(t size_class)
+      (f size_class slab_region md_bm_region md_count_v (Seq.upd (G.reveal md_region_lv) (US.v pos) 1ul))
+      (f_lemma size_class slab_region md_bm_region md_count_v (Seq.upd (G.reveal md_region_lv) (US.v pos) 1ul))
+      (SeqUtils.init_u32_refined (U32.v md_count_v))
+  )
+  (fun _ ->
+    vrefinedep
+      (vptr md_count)
+      (fun x -> U32.v x <= U32.v metadata_max == true)
+      (fun v -> left_vprop size_class slab_region md_bm_region md_region r1 r2 r3 v)
+  )
+  (requires fun h0 ->
+    sel md_count h0 == md_count_v /\
+    sel r1 h0 == idx1 /\
+    sel r2 h0 == idx2 /\
+    sel r3 h0 == idx3 /\
+    ALG.dataify (AL.v_arraylist pred1 pred2 pred3 (A.split_l md_region (u32_to_sz md_count_v)) (US.v idx1) (US.v idx2) (US.v idx3) h0) `Seq.equal` Ghost.reveal md_region_lv /\
+    Seq.index (G.reveal md_region_lv) (US.v pos) = 2ul
+  )
+  (ensures fun _ _ h1 ->
+    let blob1
+      = h1 (vrefinedep
+      (vptr md_count)
+      (fun x -> U32.v x <= U32.v metadata_max == true)
+      (fun v -> left_vprop size_class slab_region md_bm_region md_region r1 r2 r3 v)
+    ) in
+    md_count_v == dfst blob1)
+  =
+  // required for selector equality propagation
+  (**) let _ = gget (AL.varraylist pred1 pred2 pred3 (A.split_l md_region (u32_to_sz md_count_v)) (US.v idx1) (US.v idx2) (US.v idx3)) in
+  // partition improvements required
+  admit ();
+
+  let idx3' = AL.remove3 #pred1 #pred2 #pred3
+    (A.split_l md_region (u32_to_sz md_count_v))
+    (G.hide (US.v idx1)) (G.hide (US.v idx2)) idx3 pos in
+  AL.insert2 #pred1 #pred2 #pred3
+    (A.split_l md_region (u32_to_sz md_count_v))
+    idx2 (G.hide (US.v idx1)) (G.hide (US.v idx3')) pos 1ul;
+  write r3 idx3';
+  write r2 pos;
+
+  (**) pack_3 size_class slab_region md_bm_region md_region md_count r1 r2 r3
+    md_count_v (G.hide (Seq.upd (G.reveal md_region_lv) (US.v pos) 1ul))
+    idx1 pos idx3'
+
+inline_for_extraction noextract
+let deallocate_slab_aux_1_empty
+  (size_class: sc)
+  (slab_region: array U8.t{A.length slab_region = U32.v metadata_max * U32.v page_size})
+  (md_bm_region: array U64.t{A.length md_bm_region = U32.v metadata_max * 4})
+  (md_region: array AL.cell{A.length md_region = U32.v metadata_max})
+  (md_count: ref U32.t)
+  (r1 r2 r3: ref US.t)
+  (md_count_v: U32.t{U32.v md_count_v <= U32.v metadata_max})
+  (md_region_lv: G.erased (Seq.lseq AL.status (U32.v md_count_v)))
+  (idx1: US.t)
+  (idx2: US.t)
+  (idx3: US.t)
+  (pos: US.t{US.v pos < U32.v md_count_v})
+  : Steel unit
+  (
+    vptr md_count `star`
+    vptr r1 `star`
+    vptr r2 `star`
+    vptr r3 `star`
+    (AL.varraylist pred1 pred2 pred3
+      (A.split_l md_region (u32_to_sz md_count_v))
+      (US.v idx1) (US.v idx2) (US.v idx3)) `star`
+    starseq
+      #(pos:U32.t{U32.v pos < U32.v md_count_v})
+      #(t size_class)
+      (f size_class slab_region md_bm_region md_count_v (Seq.upd (G.reveal md_region_lv) (US.v pos) 0ul))
+      (f_lemma size_class slab_region md_bm_region md_count_v (Seq.upd (G.reveal md_region_lv) (US.v pos) 0ul))
+      (SeqUtils.init_u32_refined (U32.v md_count_v))
+  )
+  (fun _ ->
+    vrefinedep
+      (vptr md_count)
+      (fun x -> U32.v x <= U32.v metadata_max == true)
+      (fun v -> left_vprop size_class slab_region md_bm_region md_region r1 r2 r3 v)
+  )
+  (requires fun h0 ->
+    sel md_count h0 == md_count_v /\
+    sel r1 h0 == idx1 /\
+    sel r2 h0 == idx2 /\
+    sel r3 h0 == idx3 /\
+    ALG.dataify (AL.v_arraylist pred1 pred2 pred3 (A.split_l md_region (u32_to_sz md_count_v)) (US.v idx1) (US.v idx2) (US.v idx3) h0) `Seq.equal` Ghost.reveal md_region_lv /\
+    Seq.index (G.reveal md_region_lv) (US.v pos) = 2ul
+  )
+  (ensures fun _ _ h1 ->
+    let blob1
+      = h1 (vrefinedep
+      (vptr md_count)
+      (fun x -> U32.v x <= U32.v metadata_max == true)
+      (fun v -> left_vprop size_class slab_region md_bm_region md_region r1 r2 r3 v)
+    ) in
+    md_count_v == dfst blob1)
+  =
+  // required for selector equality propagation
+  (**) let _ = gget (AL.varraylist pred1 pred2 pred3 (A.split_l md_region (u32_to_sz md_count_v)) (US.v idx1) (US.v idx2) (US.v idx3)) in
+  // partition improvements required
+  admit ();
+
+  let idx3' = AL.remove3 #pred1 #pred2 #pred3
+    (A.split_l md_region (u32_to_sz md_count_v))
+    (G.hide (US.v idx1)) (G.hide (US.v idx2)) idx3 pos in
+  AL.insert1 #pred1 #pred2 #pred3
+    (A.split_l md_region (u32_to_sz md_count_v))
+    idx1 (G.hide (US.v idx2)) (G.hide (US.v idx3')) pos 1ul;
+  write r3 idx3';
+  write r1 pos;
+
+  (**) pack_3 size_class slab_region md_bm_region md_region md_count r1 r2 r3
+    md_count_v (G.hide (Seq.upd (G.reveal md_region_lv) (US.v pos) 0ul))
+    pos idx2 idx3'
+
+#restart-solver
+#push-options "--z3rlimit 100"
+let deallocate_slab_aux_1
   (ptr: array U8.t)
   (size_class: sc)
   (slab_region: array U8.t{A.length slab_region = U32.v metadata_max * U32.v page_size})
@@ -95,15 +219,14 @@ assume val deallocate_slab_aux_empty
   (md_count_v: U32.t{U32.v md_count_v < U32.v metadata_max})
   (md_region_lv: G.erased (Seq.lseq AL.status (U32.v md_count_v)))
   (idx1 idx2 idx3: US.t)
-  (diff: UP.t)
-  : SteelT bool
+  (pos: US.t{US.v pos < U32.v md_count_v})
+  : Steel bool
   (
     A.varray ptr `star`
     vptr md_count `star`
     vptr r1 `star`
     vptr r2 `star`
     vptr r3 `star`
-    right_vprop slab_region md_bm_region md_region md_count_v `star`
     (AL.varraylist pred1 pred2 pred3
       (A.split_l md_region (u32_to_sz md_count_v))
       (US.v idx1) (US.v idx2) (US.v idx3)) `star`
@@ -120,11 +243,212 @@ assume val deallocate_slab_aux_empty
       (vptr md_count)
       (fun x -> U32.v x <= U32.v metadata_max == true)
       (fun v ->
-         left_vprop size_class slab_region md_bm_region md_region r1 r2 r3 v `star`
-         right_vprop slab_region md_bm_region md_region v)
+         left_vprop size_class slab_region md_bm_region md_region r1 r2 r3 v)
   )
+  (requires fun h0 ->
+    let arr' = slab_array slab_region (US.sizet_to_uint32 pos) in
+    let diff = A.offset (A.ptr_of ptr) - A.offset (A.ptr_of arr') in
+    same_base_array arr' ptr /\
+    0 <= diff /\
+    diff < U32.v  page_size /\
+    (U32.v page_size) % (U32.v size_class) = 0 /\
+    sel md_count h0 == md_count_v /\
+    sel r1 h0 == idx1 /\
+    sel r2 h0 == idx2 /\
+    sel r3 h0 == idx3 /\
+    ALG.dataify (AL.v_arraylist pred1 pred2 pred3 (A.split_l md_region (u32_to_sz md_count_v)) (US.v idx1) (US.v idx2) (US.v idx3) h0) `Seq.equal` Ghost.reveal md_region_lv /\
+    Seq.index (G.reveal md_region_lv) (US.v pos) = 2ul
+  )
+  (ensures fun _ _ h1 ->
+    let blob1
+      = h1 (vrefinedep
+      (vptr md_count)
+      (fun x -> U32.v x <= U32.v metadata_max == true)
+      (fun v -> left_vprop size_class slab_region md_bm_region md_region r1 r2 r3 v)
+    ) in
+    md_count_v == dfst blob1)
+  =
+  (**) starseq_unpack_s
+    #_
+    #(pos:U32.t{U32.v pos < U32.v md_count_v})
+    #(t size_class)
+    (f size_class slab_region md_bm_region md_count_v md_region_lv)
+    (f_lemma size_class slab_region md_bm_region md_count_v md_region_lv)
+    (SeqUtils.init_u32_refined (U32.v md_count_v))
+    (US.v pos);
+  (**) SeqUtils.init_u32_refined_index (U32.v md_count_v) (US.v pos);
+  (**) change_equal_slprop
+    (f size_class slab_region md_bm_region md_count_v md_region_lv (Seq.index (SeqUtils.init_u32_refined (U32.v md_count_v)) (US.v pos)))
+    (p_full size_class (md_bm_array md_bm_region (US.sizet_to_uint32 pos), slab_array slab_region (US.sizet_to_uint32 pos)));
+  (**) p_full_unpack size_class
+    (md_bm_array md_bm_region (US.sizet_to_uint32 pos), slab_array slab_region (US.sizet_to_uint32 pos))
+    (md_bm_array md_bm_region (US.sizet_to_uint32 pos), slab_array slab_region (US.sizet_to_uint32 pos));
+  let b = deallocate_slot size_class
+    (md_bm_array md_bm_region (US.sizet_to_uint32 pos))
+    (slab_array slab_region (US.sizet_to_uint32 pos))
+    ptr in
+  if b then (
+    // deallocation success, slab no longer full
+    // TODO: is it empty?
+    let cond = deallocate_slab_aux_cond size_class
+      (md_bm_array md_bm_region (US.sizet_to_uint32 pos))
+      (slab_array slab_region (US.sizet_to_uint32 pos)) in
+    if cond then (
+      admit ();
+      allocate_slab_aux_helper size_class
+        slab_region md_bm_region md_region md_count r1 r2 r3
+        md_count_v md_region_lv pos 0ul;
+      deallocate_slab_aux_1_empty size_class
+        slab_region md_bm_region md_region md_count r1 r2 r3
+        md_count_v md_region_lv idx1 idx2 idx3 pos;
+      return b
+    ) else (
+      admit ();
+      allocate_slab_aux_helper size_class
+        slab_region md_bm_region md_region md_count r1 r2 r3
+        md_count_v md_region_lv pos 1ul;
+      deallocate_slab_aux_1_partial size_class
+        slab_region md_bm_region md_region md_count r1 r2 r3
+        md_count_v md_region_lv idx1 idx2 idx3 pos;
+      return b
+    )
+  ) else (
+    sladmit ();
+    return b
+  )
+#pop-options
 
-assume val deallocate_slab_aux_partial
+inline_for_extraction noextract
+let deallocate_slab_aux_2_empty
+  (size_class: sc)
+  (slab_region: array U8.t{A.length slab_region = U32.v metadata_max * U32.v page_size})
+  (md_bm_region: array U64.t{A.length md_bm_region = U32.v metadata_max * 4})
+  (md_region: array AL.cell{A.length md_region = U32.v metadata_max})
+  (md_count: ref U32.t)
+  (r1 r2 r3: ref US.t)
+  (md_count_v: U32.t{U32.v md_count_v <= U32.v metadata_max})
+  (md_region_lv: G.erased (Seq.lseq AL.status (U32.v md_count_v)))
+  (idx1: US.t)
+  (idx2: US.t)
+  (idx3: US.t)
+  (pos: US.t{US.v pos < U32.v md_count_v})
+  : Steel unit
+  (
+    vptr md_count `star`
+    vptr r1 `star`
+    vptr r2 `star`
+    vptr r3 `star`
+    (AL.varraylist pred1 pred2 pred3
+      (A.split_l md_region (u32_to_sz md_count_v))
+      (US.v idx1) (US.v idx2) (US.v idx3)) `star`
+    starseq
+      #(pos:U32.t{U32.v pos < U32.v md_count_v})
+      #(t size_class)
+      (f size_class slab_region md_bm_region md_count_v (Seq.upd (G.reveal md_region_lv) (US.v pos) 0ul))
+      (f_lemma size_class slab_region md_bm_region md_count_v (Seq.upd (G.reveal md_region_lv) (US.v pos) 0ul))
+      (SeqUtils.init_u32_refined (U32.v md_count_v))
+  )
+  (fun _ ->
+    vrefinedep
+      (vptr md_count)
+      (fun x -> U32.v x <= U32.v metadata_max == true)
+      (fun v -> left_vprop size_class slab_region md_bm_region md_region r1 r2 r3 v)
+  )
+  (requires fun h0 ->
+    sel md_count h0 == md_count_v /\
+    sel r1 h0 == idx1 /\
+    sel r2 h0 == idx2 /\
+    sel r3 h0 == idx3 /\
+    ALG.dataify (AL.v_arraylist pred1 pred2 pred3 (A.split_l md_region (u32_to_sz md_count_v)) (US.v idx1) (US.v idx2) (US.v idx3) h0) `Seq.equal` Ghost.reveal md_region_lv /\
+    Seq.index (G.reveal md_region_lv) (US.v pos) = 1ul
+  )
+  (ensures fun _ _ h1 ->
+    let blob1
+      = h1 (vrefinedep
+      (vptr md_count)
+      (fun x -> U32.v x <= U32.v metadata_max == true)
+      (fun v -> left_vprop size_class slab_region md_bm_region md_region r1 r2 r3 v)
+    ) in
+    md_count_v == dfst blob1)
+  =
+  // required for selector equality propagation
+  (**) let _ = gget (AL.varraylist pred1 pred2 pred3 (A.split_l md_region (u32_to_sz md_count_v)) (US.v idx1) (US.v idx2) (US.v idx3)) in
+  // partition improvements required
+  admit ();
+
+  let idx2' = AL.remove2 #pred1 #pred2 #pred3
+    (A.split_l md_region (u32_to_sz md_count_v))
+    (G.hide (US.v idx1)) idx2 (G.hide (US.v idx3)) pos in
+  AL.insert1 #pred1 #pred2 #pred3
+    (A.split_l md_region (u32_to_sz md_count_v))
+    idx1 (G.hide (US.v idx2')) (G.hide (US.v idx3)) pos 0ul;
+  write r2 idx2';
+  write r1 pos;
+
+  (**) pack_3 size_class slab_region md_bm_region md_region md_count r1 r2 r3
+    md_count_v (G.hide (Seq.upd (G.reveal md_region_lv) (US.v pos) 0ul))
+    pos idx2' idx3
+
+inline_for_extraction noextract
+let deallocate_slab_aux_2_partial
+  (size_class: sc)
+  (slab_region: array U8.t{A.length slab_region = U32.v metadata_max * U32.v page_size})
+  (md_bm_region: array U64.t{A.length md_bm_region = U32.v metadata_max * 4})
+  (md_region: array AL.cell{A.length md_region = U32.v metadata_max})
+  (md_count: ref U32.t)
+  (r1 r2 r3: ref US.t)
+  (md_count_v: U32.t{U32.v md_count_v <= U32.v metadata_max})
+  (md_region_lv: G.erased (Seq.lseq AL.status (U32.v md_count_v)))
+  (idx1: US.t)
+  (idx2: US.t)
+  (idx3: US.t)
+  (pos: US.t{US.v pos < U32.v md_count_v})
+  : Steel unit
+  (
+    vptr md_count `star`
+    vptr r1 `star`
+    vptr r2 `star`
+    vptr r3 `star`
+    (AL.varraylist pred1 pred2 pred3
+      (A.split_l md_region (u32_to_sz md_count_v))
+      (US.v idx1) (US.v idx2) (US.v idx3)) `star`
+    starseq
+      #(pos:U32.t{U32.v pos < U32.v md_count_v})
+      #(t size_class)
+      (f size_class slab_region md_bm_region md_count_v (G.reveal md_region_lv))
+      (f_lemma size_class slab_region md_bm_region md_count_v (G.reveal md_region_lv))
+      (SeqUtils.init_u32_refined (U32.v md_count_v))
+  )
+  (fun _ ->
+    vrefinedep
+      (vptr md_count)
+      (fun x -> U32.v x <= U32.v metadata_max == true)
+      (fun v -> left_vprop size_class slab_region md_bm_region md_region r1 r2 r3 v)
+  )
+  (requires fun h0 ->
+    sel md_count h0 == md_count_v /\
+    sel r1 h0 == idx1 /\
+    sel r2 h0 == idx2 /\
+    sel r3 h0 == idx3 /\
+    ALG.dataify (AL.v_arraylist pred1 pred2 pred3 (A.split_l md_region (u32_to_sz md_count_v)) (US.v idx1) (US.v idx2) (US.v idx3) h0) `Seq.equal` Ghost.reveal md_region_lv /\
+    Seq.index (G.reveal md_region_lv) (US.v pos) = 1ul
+  )
+  (ensures fun _ _ h1 ->
+    let blob1
+      = h1 (vrefinedep
+      (vptr md_count)
+      (fun x -> U32.v x <= U32.v metadata_max == true)
+      (fun v -> left_vprop size_class slab_region md_bm_region md_region r1 r2 r3 v)
+    ) in
+    md_count_v == dfst blob1)
+  =
+  (**) pack_3 size_class slab_region md_bm_region md_region md_count r1 r2 r3
+    md_count_v md_region_lv
+    idx1 idx2 idx3
+
+#restart-solver
+#push-options "--z3rlimit 100"
+let deallocate_slab_aux_2
   (ptr: array U8.t)
   (size_class: sc)
   (slab_region: array U8.t{A.length slab_region = U32.v metadata_max * U32.v page_size})
@@ -135,15 +459,14 @@ assume val deallocate_slab_aux_partial
   (md_count_v: U32.t{U32.v md_count_v < U32.v metadata_max})
   (md_region_lv: G.erased (Seq.lseq AL.status (U32.v md_count_v)))
   (idx1 idx2 idx3: US.t)
-  (diff: UP.t)
-  : SteelT bool
+  (pos: US.t{US.v pos < U32.v md_count_v})
+  : Steel bool
   (
     A.varray ptr `star`
     vptr md_count `star`
     vptr r1 `star`
     vptr r2 `star`
     vptr r3 `star`
-    right_vprop slab_region md_bm_region md_region md_count_v `star`
     (AL.varraylist pred1 pred2 pred3
       (A.split_l md_region (u32_to_sz md_count_v))
       (US.v idx1) (US.v idx2) (US.v idx3)) `star`
@@ -160,11 +483,93 @@ assume val deallocate_slab_aux_partial
       (vptr md_count)
       (fun x -> U32.v x <= U32.v metadata_max == true)
       (fun v ->
-         left_vprop size_class slab_region md_bm_region md_region r1 r2 r3 v `star`
-         right_vprop slab_region md_bm_region md_region v)
+         left_vprop size_class slab_region md_bm_region md_region r1 r2 r3 v)
   )
+  (requires fun h0 ->
+    let arr' = slab_array slab_region (US.sizet_to_uint32 pos) in
+    let diff = A.offset (A.ptr_of ptr) - A.offset (A.ptr_of arr') in
+    same_base_array arr' ptr /\
+    0 <= diff /\
+    diff < U32.v  page_size /\
+    (U32.v page_size) % (U32.v size_class) = 0 /\
+    sel md_count h0 == md_count_v /\
+    sel r1 h0 == idx1 /\
+    sel r2 h0 == idx2 /\
+    sel r3 h0 == idx3 /\
+    ALG.dataify (AL.v_arraylist pred1 pred2 pred3 (A.split_l md_region (u32_to_sz md_count_v)) (US.v idx1) (US.v idx2) (US.v idx3) h0) `Seq.equal` Ghost.reveal md_region_lv /\
+    Seq.index (G.reveal md_region_lv) (US.v pos) = 1ul
+  )
+  (ensures fun _ _ h1 ->
+    let blob1
+      = h1 (vrefinedep
+      (vptr md_count)
+      (fun x -> U32.v x <= U32.v metadata_max == true)
+      (fun v -> left_vprop size_class slab_region md_bm_region md_region r1 r2 r3 v)
+    ) in
+    md_count_v == dfst blob1)
+  =
+  (**) starseq_unpack_s
+    #_
+    #(pos:U32.t{U32.v pos < U32.v md_count_v})
+    #(t size_class)
+    (f size_class slab_region md_bm_region md_count_v md_region_lv)
+    (f_lemma size_class slab_region md_bm_region md_count_v md_region_lv)
+    (SeqUtils.init_u32_refined (U32.v md_count_v))
+    (US.v pos);
+  (**) SeqUtils.init_u32_refined_index (U32.v md_count_v) (US.v pos);
+  (**) change_equal_slprop
+    (f size_class slab_region md_bm_region md_count_v md_region_lv (Seq.index (SeqUtils.init_u32_refined (U32.v md_count_v)) (US.v pos)))
+    (p_partial size_class (md_bm_array md_bm_region (US.sizet_to_uint32 pos), slab_array slab_region (US.sizet_to_uint32 pos)));
+  (**) p_partial_unpack size_class
+    (md_bm_array md_bm_region (US.sizet_to_uint32 pos), slab_array slab_region (US.sizet_to_uint32 pos))
+    (md_bm_array md_bm_region (US.sizet_to_uint32 pos), slab_array slab_region (US.sizet_to_uint32 pos));
+  let b = deallocate_slot size_class
+    (md_bm_array md_bm_region (US.sizet_to_uint32 pos))
+    (slab_array slab_region (US.sizet_to_uint32 pos))
+    ptr in
+  if b then (
+    // deallocation success, slab no longer full
+    // TODO: is it empty?
+    let cond = deallocate_slab_aux_cond size_class
+      (md_bm_array md_bm_region (US.sizet_to_uint32 pos))
+      (slab_array slab_region (US.sizet_to_uint32 pos)) in
+    if cond then (
+      admit ();
+      (**) allocate_slab_aux_helper size_class
+        slab_region md_bm_region md_region md_count r1 r2 r3
+        md_count_v md_region_lv pos 0ul;
+      deallocate_slab_aux_2_empty size_class
+        slab_region md_bm_region md_region md_count r1 r2 r3
+        md_count_v md_region_lv idx1 idx2 idx3 pos;
+      return b
+    ) else (
+      admit ();
+      (**) allocate_slab_aux_helper size_class
+        slab_region md_bm_region md_region md_count r1 r2 r3
+        md_count_v md_region_lv pos 1ul;
+      assert (Seq.upd (G.reveal md_region_lv) (US.v pos) 1ul `Seq.equal` md_region_lv);
+    (**) starseq_weakening
+      #_
+      #(pos:U32.t{U32.v pos < U32.v md_count_v})
+      #(t size_class)
+      (f size_class slab_region md_bm_region md_count_v (Seq.upd (G.reveal md_region_lv) (US.v pos) 1ul))
+      (f size_class slab_region md_bm_region md_count_v md_region_lv)
+      (f_lemma size_class slab_region md_bm_region md_count_v (Seq.upd (G.reveal md_region_lv) (US.v pos) 1ul))
+      (f_lemma size_class slab_region md_bm_region md_count_v md_region_lv)
+      (SeqUtils.init_u32_refined (U32.v md_count_v))
+      (SeqUtils.init_u32_refined (U32.v md_count_v));
+      deallocate_slab_aux_2_partial size_class
+        slab_region md_bm_region md_region md_count r1 r2 r3
+        md_count_v md_region_lv idx1 idx2 idx3 pos;
+      return b
+    )
+  ) else (
+    sladmit ();
+    return b
+  )
+#pop-options
 
-#push-options "--compat_pre_typed_indexed_effects --z3rlimit 50"
+#push-options "--compat_pre_typed_indexed_effects --z3rlimit 100"
 let deallocate_slab'
   (ptr: array U8.t)
   (size_class: sc)
@@ -200,18 +605,20 @@ let deallocate_slab'
     vrefinedep
       (vptr md_count)
       (fun x -> U32.v x <= U32.v metadata_max == true)
-      (fun v ->
-         left_vprop size_class slab_region md_bm_region md_region r1 r2 r3 v `star`
-         right_vprop slab_region md_bm_region md_region v)
+      (size_class_vprop_aux size_class slab_region md_bm_region md_region r1 r2 r3)
   )
   (requires fun h0 ->
     let diff' = A.offset (A.ptr_of ptr) - A.offset (A.ptr_of slab_region) in
     0 <= diff' /\
+    diff' < U32.v page_size /\
     UP.v diff == diff' /\
+    same_base_array ptr slab_region /\
+    (U32.v page_size) % (U32.v size_class) = 0 /\
     sel r1 h0 == idx1 /\
     sel r2 h0 == idx2 /\
     sel r3 h0 == idx3 /\
-    md_count_v == sel md_count h0
+    md_count_v == sel md_count h0 /\
+    ALG.dataify (AL.v_arraylist pred1 pred2 pred3 (A.split_l md_region (u32_to_sz md_count_v)) (US.v idx1) (US.v idx2) (US.v idx3) h0) `Seq.equal` Ghost.reveal md_region_lv
   )
   (ensures fun _ _ _ -> True)
   =
@@ -221,52 +628,38 @@ let deallocate_slab'
   let diff_u32 = US.sizet_to_uint32 diff_sz in
   assume (U32.v diff_u32 == UP.v diff);
   let pos = U32.div diff_u32 page_size in
+  let pos' = u32_to_sz pos in
+
   // check diff/page_size < md_count
   if U32.lt pos md_count_v then (
-    let status1 = 0ul in
+    // selector equality propagation
+    let gs0 = gget (AL.varraylist pred1 pred2 pred3 (A.split_l md_region (u32_to_sz md_count_v)) (US.v idx1) (US.v idx2) (US.v idx3)) in
+    ALG.lemma_dataify_index #AL.status gs0 (U32.v pos);
+    let status1 = AL.read_in_place
+        (A.split_l md_region (u32_to_sz md_count_v))
+        (US.v idx1) (US.v idx2) (US.v idx3) (US.uint_to_t (U32.v pos)) in
     if (U32.eq status1 2ul) then (
-      sladmit ();
-      return false
-    ) else if (U32.eq status1 1ul) then (
-      let b = deallocate_slab_aux_partial ptr size_class
+      let b = deallocate_slab_aux_1 ptr size_class
         slab_region md_bm_region md_region md_count r1 r2 r3
-        md_count_v md_region_lv idx1 idx2 idx3 diff in
+        md_count_v md_region_lv idx1 idx2 idx3 pos' in
+      pack_right_and_refactor_vrefine_dep
+        size_class slab_region md_bm_region md_region md_count
+        r1 r2 r3 md_count_v;
+      return b
+    ) else if (U32.eq status1 1ul) then (
+      let b = deallocate_slab_aux_2 ptr size_class
+        slab_region md_bm_region md_region md_count r1 r2 r3
+        md_count_v md_region_lv idx1 idx2 idx3 pos' in
+      pack_right_and_refactor_vrefine_dep
+        size_class slab_region md_bm_region md_region md_count
+        r1 r2 r3 md_count_v;
       return b
     ) else (
-      let b = deallocate_slab_aux_empty ptr size_class
-        slab_region md_bm_region md_region md_count r1 r2 r3
-        md_count_v md_region_lv idx1 idx2 idx3 diff in
-      return b
+      sladmit ();
+      return false
     )
   ) else (
     sladmit ();
     return false
   )
 
-(*)
-
-    // refinement: Steel issue, does not work as logical precond
-    assume (snd b == slab_array slab_region pos);
-    // ArrayList predicate + unpacking/packing support 1/2
-    rewrite_slprop
-      emp (slab_vprop size_class (snd b) (fst b))
-      (fun _ -> admit ());
-    // metadata check done at slots level
-    let status = deallocate_slot size_class (fst b) (snd b) ptr in
-    // ArrayList predicate + unpacking/packing support 2/2
-    rewrite_slprop
-      (slab_vprop size_class (snd b) (fst b)) emp
-      (fun _ -> admit ());
-    if status then (
-      // update {partial, free, full}_slabs lists accordingly
-      sladmit ();
-      return true
-    ) else (
-      change_equal_slprop
-        (if status then emp else A.varray ptr)
-        (A.varray ptr);
-      return false
-    )
-  ) else (
-    return false
-  )
